\[
    \begin{array}{l}
        x^{-1} mod \ m \\
        \begin{tiny}
            = \begin{cases}
                \begin{array}{cl}
                    1, & \text{if} \ x=1 \\
                    -\left \lfloor\frac{m}{x} \right\rfloor(m \ mod \ x)^{-1}, & \text{otherwise}
                \end{array}
            \end{cases}(mod \ m)
        \end{tiny} \\
        \begin{tiny}
            = \begin{cases}
                \begin{array}{cl}
                    1, & \text{if} \ x=1 \\
                    (m-\left \lfloor\frac{m}{x} \right\rfloor)(m \ mod \ x)^{-1}, & \text{otherwise}
                \end{array}
            \end{cases}(mod \ m)
        \end{tiny}
    \end{array}
\]

{\raggedright
    \(若 \ p \in prime, 根據費馬小定理, 則 \) \par
    \(
        \begin{array}{rrcl}
            \because & ax & \equiv & 1 \ (mod \ p) \\
            \therefore & ax & \equiv & a^{p-1} \ (mod \ p) \\
            \therefore & x & \equiv & a^{p-2} \ (mod \ p)
        \end{array}
    \) \par
}